Challenge/Ripemd160/Submission/Proofs/Bytecode/J2RawBase.lean
@@ -113,10 +113,7 @@ theorem initResult_eq (n : Nat) : initResult n =
   rw [initResult, land224_eq_aligned _ (clamp_lt _)]
 
 def initTemplate : List Instr := [
-  .push ⟨1, by decide⟩ (UInt256.ofNat 255),
-  .push ⟨0, by decide⟩ (UInt256.ofNat 0),
-  .op .NOT,
-  .op .DIV,
+  .push ⟨32, by decide⟩ (UInt256.ofNat 0x0101010101010101010101010101010101010101010101010101010101010101),
   .op (.Dup ⟨0, by decide⟩),
   .push ⟨1, by decide⟩ (UInt256.ofNat 7),
   .op .SHL,
@@ -148,7 +145,7 @@ def initTemplate : List Instr := [
 
 def firstTemplate : List Instr := [ .op (.Dup ⟨3, by decide⟩),
     .op .ISZERO,
-    .push ⟨1, by decide⟩ (UInt256.ofNat 217),
+    .push ⟨1, by decide⟩ (UInt256.ofNat 245),
     .op .JUMPI ]
 
 def normalTemplate : List Instr := [
@@ -178,7 +175,7 @@ def normalTemplate : List Instr := [
 def normalGuardTemplate : List Instr := [ .op (.Dup ⟨3, by decide⟩),
     .op (.Dup ⟨2, by decide⟩),
     .op .LT,
-    .push ⟨1, by decide⟩ (UInt256.ofNat 188),
+    .push ⟨1, by decide⟩ (UInt256.ofNat 216),
     .op .JUMPI ]
 
 def tailTemplate : List Instr := [
@@ -201,7 +198,7 @@ def tailTemplate : List Instr := [
 def finishTemplate : List Instr := [ .op .CALLDATASIZE,
     .op (.Dup ⟨5, by decide⟩),
     .op .EQ,
-    .push ⟨2, by decide⟩ (UInt256.ofNat 292),
+    .push ⟨2, by decide⟩ (UInt256.ofNat 320),
     .op .JUMPI ]
 
 def transitionTemplate : List Instr := [ .op (.Dup ⟨9, by decide⟩),
@@ -246,14 +243,14 @@ def transitionTemplate : List Instr := [ .op (.Dup ⟨9, by decide⟩),
 def transitionGuardTemplate : List Instr := [ .op (.Dup ⟨3, by decide⟩),
     .op (.Dup ⟨2, by decide⟩),
     .op .LT,
-    .push ⟨1, by decide⟩ (UInt256.ofNat 188),
+    .push ⟨1, by decide⟩ (UInt256.ofNat 216),
     .op .JUMPI ]
 
-def toTailTemplate : List Instr := [ .push ⟨1, by decide⟩ (UInt256.ofNat 217),
+def toTailTemplate : List Instr := [ .push ⟨1, by decide⟩ (UInt256.ofNat 245),
     .op .JUMP ]
 
 def resultTemplate : List Instr := [ .op .JUMPDEST,
-    .push ⟨2, by decide⟩ (UInt256.ofNat 336),
+    .push ⟨2, by decide⟩ (UInt256.ofNat 364),
     .op .JUMPI ]
 
 
